## Linear DE's
It's of the form
$$
y' + P(x)y =Q(x)
$$
We solve it by converting into a derivative using exponentials define
$$
\mu(x) = e^{\int P(x) \, dx }
$$
then 
$$
(y' + P(x)y) \mu(x) =Q(x) \mu(x) \implies (y \mu(x) )'= Q(x)\mu(x)
$$
so
$$
y \mu(x) = \int Q(x) \mu(x) \, dx + C 
$$
 C is obtained through initial conditions.

#### What are the prerequisites for this

# Second Order Linear
For homogenous case solve the characteristic polynomial then copy the steps in the DE, it will convert to first order.

#### Non-homogenous

